while-program-infoflow/VSITypeSoundness.dfy
@@ -119,4 +119,6 @@ module VSISoundness {
         }
     }
 
+    // Finally, the Noninterference property is proved in the following
+    // 
 }
